code/experimental/P256/ecdsap256-c/Hacl_Impl_ECDSA_P256SHA256_Signature.h
@@ -12,6 +12,7 @@
 #include "Hacl_Impl_ECDSA_MM_Exponent.h"
 #include "Hacl_Impl_P256.h"
 #include "Hacl_Hash_SHA2.h"
+#include "C.h"
 #include "Hacl_Impl_ECDSA_P256SHA256_Common.h"
 #include "Hacl_Impl_ECDSA_MontgomeryMultiplication.h"
 #include "kremlib.h"
@@ -42,6 +43,25 @@ Hacl_Impl_ECDSA_P256SHA256_Signature_ecdsa_signature_step6(
   uint64_t *result
 );
 
+void Hacl_Impl_ECDSA_P256SHA256_Signature_toUint64(uint8_t *i, uint64_t *o);
+
+bool
+Hacl_Impl_ECDSA_P256SHA256_Signature_ecdsa_signature_core_nist_compliant(
+  uint8_t *m,
+  uint64_t *privKeyAsFelem,
+  uint64_t *kAsFelem,
+  uint64_t *r,
+  uint64_t *s1
+);
+
+bool
+Hacl_Impl_ECDSA_P256SHA256_Signature_ecdsa_signature_nist_compliant(
+  uint8_t *m,
+  uint8_t *privKey,
+  uint8_t *k,
+  uint8_t *result
+);
+
 bool
 Hacl_Impl_ECDSA_P256SHA256_Signature_ecdsa_signature_core(
   uint32_t mLen,
@@ -50,6 +70,15 @@ Hacl_Impl_ECDSA_P256SHA256_Signature_ecdsa_signature_core(
   uint64_t *kAsFelem,
   uint64_t *r,
   uint64_t *s1
+);
+
+bool
+Hacl_Impl_ECDSA_P256SHA256_Signature_ecdsa_signature(
+  uint32_t mLen,
+  uint8_t *m,
+  uint8_t *privKey,
+  uint8_t *k,
+  uint8_t *result
 );
 
 #define __Hacl_Impl_ECDSA_P256SHA256_Signature_H_DEFINED
